

# CALCULUS

## CHAPTER V

### Differential Equation

July, 2021.



# Outline

## 1 First-order ordinary differential equations

- Introduction
- Solving first-order ODEs

## 2 Second-order ordinary differential equation

- Introduction
- Solving 2-Linear ODE



## Discovery

*Let  $f(x) = 2x \ln x$ . Use integration by part to solve the equation  $\frac{dy}{dx} = f(x)$  for  $y$  with  $y(1) = \frac{1}{2}$ .*



## Discovery

Let  $f(x) = 2x \ln x$ . Use integration by part to solve the equation

$\frac{dy}{dx} = f(x)$  for  $y$  with  $y(1) = \frac{1}{2}$ .

$$dy = f(x)dx \implies \int dy = \int 2x \ln x dx \implies y = \int 2x \ln x dx.$$



## Discovery

Let  $f(x) = 2x \ln x$ . Use integration by part to solve the equation

$$\frac{dy}{dx} = f(x) \text{ for } y \text{ with } y(1) = \frac{1}{2}.$$

$$dy = f(x)dx \implies \int dy = \int 2x \ln x dx \implies y = \int 2x \ln x dx.$$

Let  $u' = 2x$  and  $v = \ln x$ . Then,  $u = x^2$ ,  $v' = \frac{1}{x}$  and

$$y = x^2 \ln x - \int x^2 \frac{1}{x} dx = x^2 \ln x - \int x dx = x^2 \ln x - \frac{1}{2} x^2 + c.$$

$$y(1) = 0 \implies 1 \ln 1 - \frac{1}{2} + c = \frac{1}{2} \implies c = 1. \text{ That is}$$

$$y = x^2 \left( \ln x - \frac{1}{2} \right) + 1.$$



## Discovery

Let  $f(x) = 2x \ln x$ . Use integration by part to solve the equation

$$\frac{dy}{dx} = f(x) \text{ for } y \text{ with } y(1) = \frac{1}{2}.$$

$$dy = f(x)dx \implies \int dy = \int 2x \ln x dx \implies y = \int 2x \ln x dx.$$

Let  $u' = 2x$  and  $v = \ln x$ . Then,  $u = x^2$ ,  $v' = \frac{1}{x}$  and

$$y = x^2 \ln x - \int x^2 \frac{1}{x} dx = x^2 \ln x - \int x dx = x^2 \ln x - \frac{1}{2} x^2 + c.$$

$$y(1) = 0 \implies 1 \ln 1 - \frac{1}{2} + c = \frac{1}{2} \implies c = 1. \text{ That is}$$

$$y = x^2 \left( \ln x - \frac{1}{2} \right) + 1.$$

## Definition

An equation that involves derivatives,  $\frac{d^n y}{dx^n}$ ,  $n = 1, 2, \dots$ , or differentials,  $dx, dy, \dots$ , is called an **ordinary differential equation (ODE)**.



## Remark

- The solution  $y = x^2 (\ln x - 1/2) + c$  contains an arbitrary constant  $c$ ; it is called the **general solution** of the ODE.

Whereas, the solution  $y = x^2 (\ln x - 1/2) + 1$ , that satisfies the *initial condition*  $y(1) = 1/2$  is called a **particular solution**.

## Example

Verify whether the function  $y$  is a solution of the ODE  $y'' - y = 0$ .

1)  $y = \sin x$    2)  $y = 4e^{-x}$    3)  $y = ce^x$ .



## Remark

- The solution  $y = x^2 (\ln x - 1/2) + c$  contains an arbitrary constant  $c$ ; it is called the **general solution** of the ODE.

Whereas, the solution  $y = x^2 (\ln x - 1/2) + 1$ , that satisfies the *initial condition*  $y(1) = 1/2$  is called a **particular solution**.

## Example

Verify whether the function  $y$  is a solution of the ODE  $y'' - y = 0$ .

1)  $y = \sin x$    2)  $y = 4e^{-x}$    3)  $y = ce^x$ .

*Solution:* 1) No.   2) Yes   3) Yes.

Show that  $y = cx^3$  is the general solution of the ODE  $xy' - 3y = 0$ .

Find the particular solution that satisfies the initial condition  $y(-3) = 2$ .





## Remark

• The solution  $y = x^2 (\ln x - 1/2) + c$  contains an arbitrary constant  $c$ ; it is called the **general solution** of the ODE.

Whereas, the solution  $y = x^2 (\ln x - 1/2) + 1$ , that satisfies the **initial condition**  $y(1) = 1/2$  is called a **particular solution**.

## Example

Verify whether the function  $y$  is a solution of the ODE  $y'' - y = 0$ .

1)  $y = \sin x$    2)  $y = 4e^{-x}$    3)  $y = ce^x$ .

**Solution:** 1) No.   2) Yes   3) Yes.

Show that  $y = cx^3$  is the general solution of the ODE  $xy' - 3y = 0$ .

Find the particular solution that satisfies the initial condition  $y(-3) = 2$ .

**Solution:**  $y' = 3cx^2 \implies xy' = 3cx^3 = 3y \implies xy' - 3y = 0$ ;

$y(-3) = 2 \implies c = -2/27$ ; the particular solution is  $y = -\frac{2}{27}x^3$ .



## Exercise

1) *Determine whether the function is a solution of the ODE*  
 $xy' - 2y = x^3 e^x$ .

a.  $y = x^2$    b.  $y = x^2(2 + e^x)$    c.  $y = \ln x$    d.  $y = x^2 e^x - 5x^2$ .

2) *Verify the solution of the ODE.*

a. ODE:  $3y' + 5y = -e^{-2x}$ ,  $y = e^{-2x}$

b. ODE:  $\frac{dy}{dx} = \frac{xy}{y^2 - 1}$ ,  $y^2 - 2\ln y = x^2$

c. ODE:  $y'' + 2y' + 2y = 0$ ,  $y = c_1 e^{-x} \cos x + c_2 e^{-x} \sin x$

3) *Use integration to find a general solution of the ODE.*

a.  $y' = 10x^4 - 2x^3$    b.  $y' = \frac{e^x}{4 + e^x}$    c.  $\frac{dy}{2x} = dx\sqrt{4x^2 + 1}$    d.  $y' = \tan^2 x$ .



## Definition

**A first-order ODE (1ODE) is an equation**

$$\frac{dy}{dx} = f(x, y)$$

*in which  $f(x, y)$  is a function of two variables.*



## Definition

A **first-order ODE** (1ODE) is an equation

$$\frac{dy}{dx} = f(x, y)$$

in which  $f(x, y)$  is a function of two variables.

## Remark

The order of an ODE is determined by the highest-order derivative in the equation.

## Example

Which of the equations are a first-order ODE (**1ODE**)? Find  $f(x, y)$ .

1)  $y' = x^2 + y$ ,    2)  $y'y = 2xy' - xy$ ,    3)  $\frac{dy}{x} = dx \sin x$     4)  $(xy')' = 3$ .



## Definition

A **first-order ODE** (1ODE) is an equation

$$\frac{dy}{dx} = f(x, y)$$

in which  $f(x, y)$  is a function of two variables.

## Remark

The order of an ODE is determined by the highest-order derivative in the equation.

## Example

Which of the equations are a first-order ODE (**1ODE**)? Find  $f(x, y)$ .

1)  $y' = x^2 + y$ ,    2)  $y'y = 2xy' - xy$ ,    3)  $\frac{dy}{dx} = \sin x$     4)  $(xy')' = 3$ .

**Solution:**

1) Yes,  $f = x^2 + y$     2) Yes,  $f = \frac{xy}{y-2x}$     3) Yes,  $f = \sin x$ ,    4) No.



## Definition (Separable Equation)

An ODE of the form

$$\frac{dy}{dx} = \frac{f(x)}{g(y)}$$

is called **separable** because its variables can be separated,

$$g(y)dy = f(x)dx.$$

## Remark

The separable equation can be solved by a pair of integrations:

$$\int g(y)dy = \int f(x)dx.$$



## Example

1) *Find the general solution of  $(x^2 + 4)\frac{dy}{dx} = xy$ .*



## Example

1) Find the general solution of  $(x^2 + 4) \frac{dy}{dx} = xy$ .

**Solution:**

$$1) \Rightarrow \frac{dy}{y} = \frac{x dx}{x^2 + 4} \Rightarrow \int \frac{dy}{y} = \int \frac{x dx}{x^2 + 4} \Rightarrow \ln |y| = \frac{1}{2} \ln |x^2 + 4| + c$$





## Example

1) Find the general solution of  $(x^2 + 4) \frac{dy}{dx} = xy$ .

**Solution:**

$$1) \Rightarrow \frac{dy}{y} = \frac{x dx}{x^2 + 4} \Rightarrow \int \frac{dy}{y} = \int \frac{x dx}{x^2 + 4} \Rightarrow \ln |y| = \frac{1}{2} \ln |x^2 + 4| + c$$

$$\Rightarrow \ln |y| = \frac{1}{2} \ln (x^2 + 4) + c \text{ since } x^2 + 4 \text{ is positive,}$$

$$\Rightarrow |y| = e^c \sqrt{x^2 + 4}$$

$$\Rightarrow y = \pm C \sqrt{x^2 + 4} \text{ where } C = e^c.$$



## Example

2) *Given the initial condition  $y(0) = 1$ , find the particular solution of  $xydx + e^{-x^2}(y^2 - 1)dy = 0$ .*



## Example

2) *Given the initial condition  $y(0) = 1$ , find the particular solution of  $xydx + e^{-x^2}(y^2 - 1)dy = 0$ .*

$$\begin{aligned}(2) \Rightarrow \frac{(y^2 - 1)dy}{y} &= -xe^{x^2} dx \Rightarrow \int \left(y - \frac{1}{y}\right) dy = \int -xe^{x^2} dx \\ \Rightarrow \frac{1}{2}y^2 - \ln|y| &= -\frac{1}{2}e^{x^2} + c.\end{aligned}$$



## Example

2) *Given the initial condition  $y(0) = 1$ , find the particular solution of  $xydx + e^{-x^2}(y^2 - 1)dy = 0$ .*

$$(2) \Rightarrow \frac{(y^2 - 1)dy}{y} = -xe^{x^2} dx \Rightarrow \int \left(y - \frac{1}{y}\right) dy = \int -xe^{x^2} dx$$
$$\Rightarrow \frac{1}{2}y^2 - \ln|y| = -\frac{1}{2}e^{x^2} + c.$$

*From the initial condition  $y(0) = 1$ ,  $1/2 = -1/2 + c$  which implies  $c = 1$ .*

*Thus, the solution is defined by the implicit formula*

$$\frac{1}{2}y^2 - \ln|y| = -\frac{1}{2}e^{x^2} + 1.$$



## Exercise

1) Find the equation of the curve that passes through the point  $(1,3)$  and has a slope of  $y/x^2$  at any point  $(x,y)$ .

2) The rate of change of the number of coyotes  $N(t)$  in a population is directly proportional to  $650 - N(t)$ , where  $t$  is the time in years. When  $t = 0$ , the population is 300, and  $N(2) = 500$ . Find the population when  $t = 3$ .

3) Solve the logistic ODE  $y' = ky\left(1 - \frac{y}{L}\right)$ .

4) Find the general solution of the ODE.

a.  $y \ln x - xy' = 0$    b.  $\sqrt{x} + y' \sqrt{y} = 0$    c.  $\frac{u}{v} = uv \sin v^2$ .

5) Find the orthogonal trajectories of the family.

a.  $x^2 + y^2 = c$    b.  $y^2 = 2cx$    c.  $y = ce^x$



## Definition

*Equations of the form*

$$y' + p(x)y = q(x)$$

*are called **first-order linear ODEs**.*

*The general solution of this differential equation is*

$$yu = \int q u dx + c$$

*where  $u = e^{\int p(x) dx}$  is called the **integrating factor** since its presence makes the equation integrable.*



## Definition

*Equations of the form*

$$y' + p(x)y = q(x)$$

*are called **first-order linear ODEs**.*

*The general solution of this differential equation is*

$$yu = \int qu dx + c$$

*where  $u = e^{\int p(x) dx}$  is called the **integrating factor** since its presence makes the equation integrable.*

## Remark

*The equation  $y' + p(x)y = q(x)$  is linear in  $y$  because  $y$  and its derivative  $y'$  occur only to the first power, and they are not multiplied together.*



## Example

1) *Determine whether the differential equation is linear. Explain your reasoning. If YES then write the equation in the standard form  $y' + py = q$ .*

a.  $x^3y' + xy = e^x + 1$       b.  $2xy - y'\ln x = y$

c.  $y' - y\sin x = xy^2$       d.  $\frac{2 - y'}{y} = 5x.$





## Example

1) *Determine whether the differential equation is linear. Explain your reasoning. If YES then write the equation in the standard form  $y' + py = q$ .*

a.  $x^3y' + xy = e^x + 1$       b.  $2xy - y' \ln x = y$

c.  $y' - y \sin x = xy^2$       d.  $\frac{2 - y'}{y} = 5x$ .

**Solution:**

a. YES,  $y' + \frac{1}{x^2}y = \frac{e^x + 1}{x^3}$

b. YES,  $y' - \frac{2x}{\ln x}y = -\frac{y}{\ln x}$

c. NO, because of  $y^2$ .

d. YES,  $y' + 5xy = 2$



## Example

*Solve the equation*

$$1) \ y' - \frac{3}{x}y = x, x > 0 \quad 2) \ y' - \frac{1}{3x}y = \frac{\ln x + 1}{3x}$$



## Example

*Solve the equation*

$$1) \ y' - \frac{3}{x}y = x, x > 0 \quad 2) \ y' - \frac{1}{3x}y = \frac{\ln x + 1}{3x}$$

### Solution:

*Since  $p(x) = -3/x$ , the integrating factor is*

$$u(x) = e^{\int p(x) dx} = e^{\int \frac{-3}{x} dx} = e^{-3 \ln |x|} = e^{-3 \ln x} = x^{-3} \text{ since } x > 0.$$



## Example

*Solve the equation*

$$1) \ y' - \frac{3}{x}y = x, x > 0 \quad 2) \ y' - \frac{1}{3x}y = \frac{\ln x + 1}{3x}$$

### Solution:

*Since  $p(x) = -3/x$ , the integrating factor is*

$$u(x) = e^{\int p(x)dx} = e^{\int \frac{-3}{x}dx} = e^{-3\ln|x|} = e^{-3\ln x} = x^{-3} \text{ since } x > 0.$$

$$yu = \int qu dx \implies yx^{-3} = \int x\dot{x}^{-3}dx = \int x^{-2}dx = -x^{-1} + c.$$

*Therefore,  $y = -x^2 + cx^3, x > 0$ .*



## Example

$$2) \ y' - \frac{1}{3x}y = \frac{\ln x + 1}{3x}, x > 0.$$



## Example

$$2) \ y' - \frac{1}{3x}y = \frac{\ln x + 1}{3x}, x > 0.$$

**Solution:**

$$p(x) = -\frac{1}{3x} \implies u = e^{\int p(x)dx} = \exp\left(-\frac{1}{3} \int \frac{dx}{x}\right) = \exp\left(-\frac{1}{3} \ln|x|\right)$$



## Example

$$2) \quad y' - \frac{1}{3x}y = \frac{\ln x + 1}{3x}, x > 0.$$

### Solution:

$$p(x) = -\frac{1}{3x} \implies u = e^{\int p(x)dx} = \exp\left(-\frac{1}{3} \int \frac{dx}{x}\right) = \exp\left(-\frac{1}{3} \ln|x|\right) \\ = \exp(\ln x^{-1/3}) = x^{-1/3}$$

$$\text{and } uy = \int \frac{\ln x + 1}{3x} u dx \implies yx^{-1/3} = \frac{1}{3} \int x^{-4/3} (1 + \ln x) dx$$



## Example

$$2) \quad y' - \frac{1}{3x}y = \frac{\ln x + 1}{3x}, \quad x > 0.$$

### Solution:

$$p(x) = -\frac{1}{3x} \implies u = e^{\int p(x)dx} = \exp\left(-\frac{1}{3} \int \frac{dx}{x}\right) = \exp\left(-\frac{1}{3} \ln|x|\right) \\ = \exp(\ln x^{-1/3}) = x^{-1/3}$$

$$\text{and } uy = \int \frac{\ln x + 1}{3x} u dx \implies yx^{-1/3} = \frac{1}{3} \int x^{-4/3} (1 + \ln x) dx$$

Integration by parts of the RHS,  $\frac{1}{3} \int x^{-4/3} (1 + \ln x) dx$  (by setting

$w' = x^{-4/3}$  and  $v = 1 + \ln x$  and considering  $\int w'v = wv - \int wv'$ ),  
leads to the solution





## Example

$$2) \quad y' - \frac{1}{3x}y = \frac{\ln x + 1}{3x}, x > 0.$$

### Solution:

$$p(x) = -\frac{1}{3x} \implies u = e^{\int p(x)dx} = \exp\left(-\frac{1}{3} \int \frac{dx}{x}\right) = \exp\left(-\frac{1}{3} \ln|x|\right) \\ = \exp(\ln x^{-1/3}) = x^{-1/3}$$

$$\text{and } uy = \int \frac{\ln x + 1}{3x} u dx \implies yx^{-1/3} = \frac{1}{3} \int x^{-4/3} (1 + \ln x) dx$$

*Integration by parts of the RHS,  $\frac{1}{3} \int x^{-4/3} (1 + \ln x) dx$  (by setting*

*$w' = x^{-4/3}$  and  $v = 1 + \ln x$  and considering  $\int w'v = wv - \int wv'$ ),*  
*leads to the solution*

$$y = x^{1/3} \left( -x^{-1/3} (\ln x + 1) + \int x^{-4/3} dx + c \right) \\ = x^{1/3} \left( -x^{-1/3} (\ln x + 1) - 3x^{-1/3} + c \right) \\ = cx^{1/3} - \ln x - 4.$$



## Exercise

*Solve the following differential equations.*

1)  $xy' + y = e^x, x > 0$

2)  $e^x y' + 2e^x y = 1$

3)  $xy' + 3y = \frac{\sin x}{x^2}, x > 0$

4)  $y' + y \tan x = \cos^2 x, -\frac{\pi}{2} < x < \frac{\pi}{2}$

5)  $xy' - y = 2x \ln x$

6)  $\theta \frac{dy}{d\theta} - 2y = \theta^3 \sec \theta \tan \theta, \theta > 0, y(\pi/3) = 2$

7)  $(x+1)y' - 2(x^2 + x)y = \frac{e^x}{x+1}, x > -1, y(0) = 5.$



# Outline

## 1 First-order ordinary differential equations

- Introduction
- Solving first-order ODEs

## 2 Second-order ordinary differential equation

- Introduction
- Solving 2-Linear ODE



So far, all the equations have been first order ODEs. Now we will turn to higher-order equations; in particular, second-order equation with constant coefficients.

## Definition

☛ In general a **second order ODE** involves  $\frac{d^2y}{dx^2}$ ,  $\frac{dy}{dx}$ ,  $y$  and  $x$ .



So far, all the equations have been first order ODEs. Now we will turn to higher-order equations; in particular, second-order equation with constant coefficients.

## Definition

☛ In general a **second order ODE** involves  $\frac{d^2y}{dx^2}$ ,  $\frac{dy}{dx}$ ,  $y$  and  $x$ .

☛ A second-order **linear** ODE is

$$a(x)y'' + b(x)y' + c(x)y = d(x) \text{ where } a(x) \neq 0.$$



So far, all the equations have been first order ODEs. Now we will turn to higher-order equations; in particular, second-order equation with constant coefficients.

## Definition

☛ In general a **second order ODE** involves  $\frac{d^2y}{dx^2}$ ,  $\frac{dy}{dx}$ ,  $y$  and  $x$ .

☛ A second-order **linear** ODE is

$$a(x)y'' + b(x)y' + c(x)y = d(x) \text{ where } a(x) \neq 0.$$

☛ A second-order linear ODE **with constant coefficients** is of the form

$$ay'' + by' + cy = d(x)$$

where  $a \neq 0$ ,  $b$  and  $c$  are constant real numbers.



So far, all the equations have been first order ODEs. Now we will turn to higher-order equations; in particular, second-order equation with constant coefficients.

## Definition

☛ In general a **second order ODE** involves  $\frac{d^2y}{dx^2}$ ,  $\frac{dy}{dx}$ ,  $y$  and  $x$ .

☛ A second-order **linear** ODE is

$$a(x)y'' + b(x)y' + c(x)y = d(x) \text{ where } a(x) \neq 0.$$

☛ A second-order linear ODE **with constant coefficients** is of the form

$$ay'' + by' + cy = d(x)$$

where  $a \neq 0$ ,  $b$  and  $c$  are constant real numbers.

☛ The equation is said to be **homogeneous** if  $d(x) = 0$ . That is

$$ay'' + by' + cy = 0.$$



## Solving a second-order homogeneous ODE with constant coefficients

Suppose we want to solve  $ay'' + by' + c = 0$ , with  $a \neq 0$ .





## Solving a second-order homogeneous ODE with constant coefficients

Suppose we want to solve  $ay'' + by' + c = 0$ , with  $a \neq 0$ .

Assuming that the solution is on the form  $y = e^{rx}$ , then  $y' = re^{rx}$

and  $y'' = r^2 e^{rx}$  so that the equation becomes

$$ay'' + by' + c = ar^2 e^{rx} + bre^{rx} + ce^{rx} = (ar^2 + br + c)e^{rx}.$$



## Solving a second-order homogeneous ODE with constant coefficients

Suppose we want to solve  $ay'' + by' + c = 0$ , with  $a \neq 0$ .

Assuming that the solution is on the form  $y = e^{rx}$ , then  $y' = re^{rx}$  and  $y'' = r^2 e^{rx}$  so that the equation becomes

$$ay'' + by' + c = ar^2 e^{rx} + bre^{rx} + ce^{rx} = (ar^2 + br + c)e^{rx}.$$

In other words,  $ay'' + by' + c = 0$  yields  $ar^2 + br + c = 0$ .

### Definition

$$ar^2 + br + c = 0$$

*is called the **characteristic polynomial** of the ODE*

$$ay'' + by' + c = 0.$$



The roots of the characteristic polynomial determine the solutions of the homogeneous ODE.

## Property

### ☛ Real and distinct roots.

*If we denote the roots by  $r_1$  and  $r_2$ , then the general solution of the ODE is*

$$y = c_1 e^{r_1 x} + c_2 e^{r_2 x} \text{ where } c_1, c_2 \in \mathbb{R}.$$



The roots of the characteristic polynomial determine the solutions of the homogeneous ODE.

## Property

### ☛ Real and distinct roots.

*If we denote the roots by  $r_1$  and  $r_2$ , then the general solution of the ODE is*

$$y = c_1 e^{r_1 x} + c_2 e^{r_2 x} \text{ where } c_1, c_2 \in \mathbb{R}.$$

### ☛ Real and identical roots.

*If we denote the double root by  $r_1$ , then the general solution of the ODE is*

$$y = (c_1 + c_2 x) e^{r_1 x} \text{ where } c_1, c_2 \in \mathbb{R}.$$



The roots of the characteristic polynomial determine the solutions of the homogeneous ODE.

## Property

### ☛ Real and distinct roots.

If we denote the roots by  $r_1$  and  $r_2$ , then the general solution of the ODE is

$$y = c_1 e^{r_1 x} + c_2 e^{r_2 x} \text{ where } c_1, c_2 \in \mathbb{R}.$$

### ☛ Real and identical roots.

If we denote the double root by  $r_1$ , then the general solution of the ODE is

$$y = (c_1 + c_2 x) e^{r_1 x} \text{ where } c_1, c_2 \in \mathbb{R}.$$

### ☛ Complex and distinct roots.

If we denote the roots by  $r_1 = \alpha + i\beta$  and  $r_2 = \alpha - i\beta$ , then the general solution of the ODE is

$$y = (c_1 \cos \beta + c_2 \sin \beta) e^{\alpha x} \text{ where } c_1, c_2 \in \mathbb{R}.$$



## Example

*Solve (1)  $2y'' + 7y' = 4y$ , and (2)  $y'' + 2y' + y = 0$ .*



## Example

Solve (1)  $2y'' + 7y' = 4y$ , and (2)  $y'' + 2y' + y = 0$ .

## Solution

(1) The characteristic polynomial of  $2y'' + 7y' - 4y = 0$  is  $2r^2 + 7r - 4 = 0$ . The discriminant  $\Delta = b^2 - 4ac = 49 + 32 = 81 > 0$  yields two distinct real roots  $r_{1,2} = \frac{-b \pm \sqrt{\Delta}}{2a} = -4, \frac{1}{2}$ .

Thus, the general solution is  $y = c_1 e^{-4x} + c_2 e^{\frac{x}{2}}$ .



## Example

Solve (1)  $2y'' + 7y' = 4y$ , and (2)  $y'' + 2y' + y = 0$ .

## Solution

(1) The characteristic polynomial of  $2y'' + 7y' - 4y = 0$  is  $2r^2 + 7r - 4 = 0$ . The discriminant  $\Delta = b^2 - 4ac = 49 + 32 = 81 > 0$  yields two distinct real roots  $r_{1,2} = \frac{-b \pm \sqrt{\Delta}}{2a} = -4, \frac{1}{2}$ .

Thus, the general solution is  $y = c_1 e^{-4x} + c_2 e^{\frac{x}{2}}$ .

(2) The characteristic polynomial is  $r^2 + 2r + 1 = (r + 1)^2$ . We get a double real root  $r_1 = -1$ .

Thus  $y = (c_1 + c_2 x) e^{-x}$ .

